coq-osiris/theories/test/test.v
@@ -37,7 +37,7 @@ Local Notation crashes e :=
 (* The construct [EAssert e] is evaluated as a choice between skipping the
    dynamic test and performing the dynamic test (eval.v). Here, we want the
    dynamic tests to be performed, so we choose the right-hand side. This is
-   done by using [StepChooseRight]. It is brittle, but should do for now. *)
+   done by using [StepFlip false]. It is brittle, but should do for now. *)
 
 Lemma is_fresh :
   ∀ (σ : store), σ !! (fresh (dom σ)) = None.
@@ -51,7 +51,7 @@ Local Ltac step :=
   first [
       eapply StepEval
     | eapply StepLoop
-    | eapply StepChooseRight
+    | eapply (StepFlip false)
     | eapply StepParRetRet
     | eapply StepParLeft; [ step ]
     | eapply StepParRight; [ step ]
